Looking at noninterference for the ctx

io/IIO.Behavior.fst
@@ -8,29 +8,88 @@ open IIO
 
 assume val __reify_IIOwp (#a:Type) (#wp:Hist.hist a) (#fl:tflag) ($f:unit -> IIOwp a fl wp) : GTot (dm_giio a fl wp)
 
-(* We define `beh` that returns the set of traces produced by a whole program.
-   Since whole programs start with the empty trace, 
-   the local trace contains the complete trace.
+(** Confusing elements:
+1) there are two definitions of trace. one from IIO.Sig.trace and one from BeyondCriteria.trace
+2) prefixed_trace_property may be confusing 
+**)
+
+type prefixed_trace_property (pre:IIO.Sig.trace -> Type0) = h:IIO.Sig.trace -> (#_:squash (pre h)) -> BeyondCriteria.trace #event -> Type0
+
+(* We define `beh_giio` that returns the set of traces produced by a program
+   starting from a given history `h`.
 
    `theta` is a weakest precondtion monad, and we need it to be
    a post-condition. Looking at Kenji's thesis, we can apply the
    'backward predicate transformer 2.3.4' and the 
    'pre-/postcondition transformer 2.3.2' to obtain
    the 'set' of traces produces by the whole program. *)
-val beh_giio : dm_giio int AllActions trivial_hist -> trace_property #event
-let beh_giio ws tr =
+val beh_giio : #pre:(trace -> Type0) -> #fl:erased tflag -> dm_giio int fl (to_hist pre (fun _ _ _ -> True)) -> prefixed_trace_property pre 
+let beh_giio ws h tr =
   match tr with
   | Infinite_trace _ -> False
   | Finite_trace lt res -> 
-   (* We verify specs of whole programs, thus, instead of having
-      properties forall histories, we can specialize it for the
-      empty history *)
-    forall p. dm_giio_theta ws p [] ==> p lt res
+    forall p. dm_giio_theta ws p h ==> p lt res
 
+(* _beh is used on whole programs, thus, 
+   we specialize it with the empty history *)
 val _beh : (unit -> IIO int AllActions (fun _ -> True) (fun _ _ _ -> True)) -> trace_property #event
 let _beh ws =
-  beh_giio (__reify_IIOwp ws) 
+  beh_giio (__reify_IIOwp ws) []
 
 irreducible
 val beh : (unit -> IIO int AllActions (fun _ -> True) (fun _ _ _ -> True)) ^-> trace_property #event
 let beh = on_domain _ (fun ws -> _beh ws)
+
+val _beh_ctx : #pre:(trace -> Type0) -> (unit -> IIO int AllActions pre (fun _ _ _ -> True)) -> prefixed_trace_property pre 
+let _beh_ctx ws h =
+  beh_giio (__reify_IIOwp ws) h 
+
+//irreducible
+val beh_ctx : #pre:(trace -> Type0) -> (unit -> IIO int AllActions pre (fun _ _ _ -> True)) ^-> prefixed_trace_property pre 
+let beh_ctx #pre = on_domain _ (fun ws -> _beh_ctx #pre ws)
+
+type prefixed_trace (pre:trace->Type0) = h:trace{pre h} * BeyondCriteria.trace #event  
+
+let mem (#pre:trace->Type0) ((h, tr):prefixed_trace pre) (s1:prefixed_trace_property pre) =
+  s1 h tr
+
+open FStar.Tactics
+
+val lemma0 : #pre:(trace -> Type0) -> ctx:(fl:erased tflag -> unit -> IIO int fl pre (fun _ _ _ -> True)) -> h1:trace{pre h1} -> h2:trace{pre h2} -> tr:BeyondCriteria.trace -> Lemma (
+  let reified_ctx = __reify_IIOwp (ctx AllActions) in
+  beh_giio #pre reified_ctx h1 tr ==> beh_giio #pre reified_ctx h2 tr
+)
+
+let lemma0 #pre ctx h1 h2 tr =
+  let reified_ctx = __reify_IIOwp (ctx AllActions) in
+  introduce beh_giio #pre reified_ctx h1 tr 
+  ==> beh_giio #pre reified_ctx h2 tr 
+  with _. begin
+    assume (beh_giio #pre reified_ctx h2 tr)
+  end
+
+(* h is non-interfering for flag polymorphic ctx
+  -- should be true since a flag polymorphic ctx can do no actions *)
+val test : #pre:(trace -> Type0) -> ctx:(fl:erased tflag -> unit -> IIO int fl pre (fun _ _ _ -> True)) ->
+  Lemma (
+    let bh = beh_ctx #pre (ctx AllActions) in
+    forall t1 t2. t1 `mem` bh /\ t2 `mem` bh ==>
+      (exists t3. t3 `mem` bh /\ fst t1 == fst t3 /\ snd t2 == snd t3))
+
+let test #pre ctx = 
+  let bh = beh_ctx #pre (ctx AllActions) in
+  let reified_ctx : dm_giio int AllActions (to_hist pre (fun _ _ _ -> True)) = __reify_IIOwp (ctx AllActions) in
+  introduce forall (t1 t2:prefixed_trace pre).
+  t1 `mem` bh /\ t2 `mem` bh 
+  ==> (exists (t3:prefixed_trace pre). t3 `mem` bh /\ fst t1 == fst t3 /\ snd t2 == snd t3) 
+  with begin
+    introduce t1 `mem` bh /\ t2 `mem` bh
+    ==> (exists (t3:prefixed_trace pre). t3 `mem` bh /\ fst t1 == fst t3 /\ snd t2 == snd t3)
+    with _. begin
+      let t3 : prefixed_trace pre = (fst t1, snd t2) in 
+      assert (t2 `mem` bh);
+      lemma0 #pre ctx (fst t2) (fst t1) (snd t2);
+      assert (beh_giio #pre reified_ctx (fst t2) (snd t2) ==> beh_giio #pre reified_ctx (fst t1) (snd t2));
+      assert (t3 `mem` bh)
+    end
+  end
